slide_geq_sorted

sort/simplest01.v
@@ -20,12 +20,11 @@ Proof. move=> i [a l]; done. Qed.
 Lemma slide_hold_length : forall i l, 
   length l = length (snd (slide i l)).
 Proof.
-  fix slide_hold_length 2. move=> i [| a l']; rewrite /=. done.
+  fix slide_hold_length 2. move=> i [| a l'] /=. done.
   case H : (i < a); rewrite snd_destr_comm /=; apply f_equal, slide_hold_length.
 Qed.
 
-Program Fixpoint sort' (l1:list nat) (l2:list nat) {measure (length l2)} 
-: (list nat) * (list nat):=
+Program Fixpoint sort' l1 l2 {measure (length l2)} : list nat * list nat:=
   match l2 with
   | [] => (l1, [])
   | h :: t => match slide h l1 with
@@ -84,11 +83,7 @@ Proof.
     rewrite slide_cons. by rewrite indep_prod. apply (cons_cons_sorted _ _ _ S).
 Qed.
 
-Lemma leq_cons_sorted : forall a h l, 
-  sorted (h :: l) -> a <= h -> sorted (a :: h :: l).
-Proof. move=> a h [|n l'] S H; apply sorted_cons; [apply H|apply sorted_1|apply H|apply S]. Qed.
-
-Lemma leq_all_cons_sorted : forall a i l, 
+Lemma leq_all_cons_sorted' : forall a i l, 
   sorted (a :: l) -> a <= i -> 
   sorted (let (h, t) := slide i l in t ++ [h]) ->
   sorted (let (h, t) := slide i l in a :: t ++ [h]).
@@ -105,14 +100,22 @@ Lemma slide_sorted' : forall a l, sorted l ->
 Proof.
   fix slide_sorted' 2.
   move=> a [|h t] S /=. apply sorted_1. case H: (a < h); rewrite 2!indep_prod /=;
-  rewrite -(indep_prod _ _ _ (fun w1 w2 => _ :: w2 ++ [w1])); apply leq_all_cons_sorted.
-   - apply (cons_cons_sorted _ h _), (leq_cons_sorted _ _ _ S), ltnW, H.  
+  rewrite -(indep_prod _ _ _ (fun w1 w2 => _ :: w2 ++ [w1])); apply leq_all_cons_sorted'.
+   - apply (cons_cons_sorted _ h _), (fun Hw => sorted_cons _ _ _ Hw S), ltnW, H.  
    - apply ltnW, H.
    - apply slide_sorted', (cons_sorted _ _ S).
    - apply S.
    - move:H. rewrite ltnNge. by move/eqP/eqP.
    - apply slide_sorted', (cons_sorted _ _ S).
-Qed. 
+Qed.
+
+Corollary leq_all_cons_sorted : forall a i l, 
+  sorted (a :: l) -> a <= i -> 
+  sorted (let (h, t) := slide i l in a :: t ++ [h]).
+Proof.
+  move=> a i l S Hle. apply leq_all_cons_sorted'. apply S. apply Hle.
+  apply slide_sorted'. apply (cons_sorted _ _ S).
+Qed.
 
 Lemma app_cons_comm : forall A (l1:list A) n l2, 
   l1 ++ n :: l2 = (l1 ++ [n]) ++ l2.
@@ -128,12 +131,58 @@ Qed.
 Lemma app_sorted : forall l1 l2, sorted (l1 ++ l2) -> sorted l1.
 Proof.
   fix app_sorted 2.
-  move => l1 [|n l2].
-  (* intros l1. destruct l2. *)
-  by rewrite app_nil_r.
+  move => l1 [|n l2]. by rewrite app_nil_r.
   rewrite app_cons_comm => S. pose (app_sorted _ _ S) as S2.
   by apply sorted_snoc in S2.
 Qed.
+
+Corollary leq_all_cons_sorted_snd : forall a i l,
+  sorted (a :: l) -> a <= i -> sorted (a :: snd (slide i l)).
+Proof.
+  move=> a i l S Hle. move: (leq_all_cons_sorted _ _ _ S Hle).
+  rewrite indep_prod app_comm_cons. apply app_sorted.
+Qed.
+
+Lemma sorted_trans_cons_cons : forall l a b,
+  sorted (l ++ [a]) -> sorted (a :: [b]) -> sorted (l ++ [a] ++ [b]).
+Proof.
+  induction l. done. induction l. move=> /= a0 b S1 S2.
+  apply sorted_cons. inversion S1. apply H1. apply S2.
+  move:IHl IHl0 => /= IHl IHl0 a1 b S1 S2. apply sorted_cons. inversion S1.
+  apply H1. inversion S1. apply IHl. apply H3. apply S2.
+Qed.
+
+Lemma sorted_trans_cons: forall a h t l3,
+  sorted (a :: h :: t) -> sorted (h :: t ++ l3) -> sorted (a :: h :: t ++ l3).
+Proof.
+  move=> /= a h t l3 S1 S2. apply sorted_cons. inversion S1. apply H1.
+  apply S2.
+Qed.
+
+Lemma sorted_trans_app_app: forall l1 h t l3,
+  sorted (l1 ++ h :: t) -> sorted (h :: t ++ l3) -> sorted (l1 ++ h :: t ++ l3).
+Proof.
+  induction l1. done.
+  destruct l1. apply sorted_trans_cons.
+  move:IHl1 => /= IHl1 h t l3 S1 S2. inversion S1.
+  apply sorted_cons. apply H1. apply IHl1. 
+  apply H3. apply S2.
+Qed. 
+
+(*
+Lemma sorted_trans_app_snoc : forall l1 l2 b, l2 <> [] ->
+  sorted (l1 ++ l2) -> sorted (l2 ++ [b]) -> sorted (l1 ++ l2 ++ [b]).
+Proof.
+  induction l2. done. move=> /= b _ S1 S2.
+  induction l1. done. induction l1.
+  move=> l1 l2 b S1 S2. 
+
+Lemma sorted_trans : forall l1 l2 l3,
+  sorted (l1 ++ l2) -> sorted (l2 ++ l3) -> sorted (l1 ++ l2 ++ l3).
+Proof.
+  induction l1. done. induction l1; move: IHl1=> /= IHl1 l2 l3 S1 S2.
+
+  case l2. rewrite /=.  *)
 
 Lemma slide_sorted : forall a l, sorted l -> sorted (snd (slide a l)).
 Proof. 
@@ -141,11 +190,116 @@ Proof.
   rewrite indep_prod. apply app_sorted.
 Qed.
 
-(* Lemma sort'_sorted : forall l1 l2, sorted l1 -> sorted (fst (sort' l1 l2)).
+Lemma slide_leq : forall i l, i <= fst (slide i l).
+Proof.
+  fix slide_leq 2.
+  move => i [|h t] => /=. done. case H: (i < h); rewrite indep_prod /=.
+  apply (leq_trans (n := h)). apply ltnW, H. apply slide_leq.
+  apply slide_leq.
+Qed.
+
+Lemma slide_geq_sorted : forall i l j, sorted l ->
+  let (i', l') := slide i l in (i' <= j -> sorted (l' ++ [j])).
+Proof.
+  move => i l j. rewrite indep_prod. move: l i j. induction l.
+  move=> i j S Hle; apply sorted_1. move: a.
+  
+  move=> a i j S /=. 
+  rewrite 2! indep_prod. 
+  destruct l; case H: (i < a) => /= Hle.
+   - apply sorted_cons. apply (leq_trans(n:=a)). apply ltnW, H. apply Hle. apply sorted_1.
+   - apply sorted_cons. apply (leq_trans(n:=i)). move:H.
+    rewrite ltnNge. move/eqP/eqP. done. apply Hle. apply sorted_1.
+   - move:Hle. rewrite 2!indep_prod. case H2: (a < n) => /= Hle.
+     - apply sorted_cons. apply ltnW, H. 
+      rewrite app_comm_cons. 
+      inversion S. assert (fst (slide a (n :: l)) = fst (slide n l)).
+      { rewrite /=. case H2': (a < n); rewrite indep_prod /=. done. 
+        rewrite H2' in H2. inversion H2. }
+      rewrite -H6 in Hle.
+      pose (IHl a j H5 Hle). assert (snd (slide a (n :: l)) = a :: snd (slide n l)).
+      { rewrite /=. case H2': (a < n); rewrite indep_prod /=. done.
+        rewrite H2' in H2. inversion H2. }
+      rewrite -H7. apply s.
+    - inversion S. move:IHl S. case (leq_lt _ _ H2 H3) => /= IHl S.
+      apply sorted_cons. apply ltnW, H. inversion S. 
+      move:(IHl a j H10). case H': (a < a). rewrite ltnn in H'.
+      inversion H'. rewrite indep_prod /=. apply. apply Hle.
+  - move:Hle. rewrite 2!indep_prod. case H2: (i < n) => /= Hle.
+    - apply sorted_cons. move: H. rewrite ltnNge. move/eqP/eqP. done.
+      inversion S. assert (fst (slide i (n :: l)) = fst (slide n l)).
+      { rewrite /=. case H2': (i < n); rewrite indep_prod /=. done.
+        rewrite H2' in H2. inversion H2. }
+      assert (snd (slide i (n :: l)) = i :: snd (slide n l)).
+      { rewrite /=. case H2': (i < n); rewrite indep_prod /=. done.
+        rewrite H2' in H2. inversion H2. }
+      rewrite app_comm_cons -H7. apply IHl. apply H5.
+      rewrite H6. apply Hle.
+    - apply sorted_cons. inversion S. apply H3.
+      inversion S. assert (fst (slide i l) = fst (slide i (n :: l))).
+      { rewrite /=. case H2': (i < n); rewrite indep_prod /=. rewrite H2' in H2.
+        inversion H2. done. }
+      assert (n :: snd (slide i l) = snd (slide i (n :: l))).
+      { rewrite /=. case H2': (i < n); rewrite indep_prod /=. rewrite H2' in H2.
+        inversion H2. done. }
+      rewrite app_comm_cons H7. apply IHl. apply H5. rewrite -H6. apply Hle.
+    Qed.
+
+    case e.
+   apply sorted_cons. apply (leq_trans(n:=a)). apply ltnW, H.
+    
+    assert (sorted (snd (slide a l) ++ [j])).
+    { apply IHl. apply (cons_sorted _ _ S). apply Hle. }
+    destruct l. rewrite /=. apply sorted_cons. inversion Hle.
+    apply (leq_trans(n:=a)). apply ltnW, H. apply H2.
+    apply sorted_1. rewrite /= 2!indep_prod. case H2: (a < n).
+    rewrite /=. apply sorted_cons. apply ltnW, H.
+    apply 
+    Check leq_all_cons_sorted_snd.
+
+  induction l.
+  move=> a i j S /=. case H: (i < a) => /= Hle. 
+   - apply sorted_cons. apply (leq_trans(n:=a)). apply ltnW, H. apply Hle.
+   - apply sorted_1.
+   - apply sorted_cons. move: H. rewrite ltnNge. move/eqP/eqP => H.
+    apply (leq_trans(n:=i)). apply H. apply Hle.
+   - apply sorted_1.
+   - move=> a0 i j S /=. rewrite 6!indep_prod. case H: (i < a0).
+     - case H2: (a0 < a) => /= Hle.
+       - apply sorted_cons. apply ltnW, H. pose (cons_sorted _ _ S).
+        pose ()
+  
+  move=> a i j S /=. rewrite 2! indep_prod. case H: (i < a) => /= Hle.
+
+
+  induction l.
+   - move=> a i j /=. case H: (i < a) => /= Hle; apply sorted_cons.
+    apply (leq_trans(n:=a)). apply ltnW, H. apply Hle. apply sorted_1.
+    move: H. rewrite ltnNge. move/eqP/eqP => H. apply (leq_trans(n:=i)).
+    apply H. apply Hle. apply sorted_1.
+   - move=> a0 i j /=. rewrite 6!indep_prod. 
+  case H: (i < a0) => /=. case H2: (a0 < a) => /= Hle.
+  apply sorted_cons. apply ltnW, H. apply 
+  rewrite 2!indep_prod. induction l. case H: (i < a) => /= Hle. induction l.
+   - 
+
+
+  fix slide_geq_sorted 2.
+  move=> i [|h t] j. move=> H; apply sorted_1.
+  rewrite /= 3!indep_prod. case H: (i < h) => /= Hle.
+  induction t. rewrite /=. rewrite /= in Hle. apply sorted_cons.
+  apply (leq_trans(n := h)). apply ltnW, H. apply Hle.
+  apply sorted_1.
+  rewrite /= 2!indep_prod. case H2: (h < a) => /=. apply sorted_cons.
+  apply ltnW, H. apply IHt.
+  apply 
+
+Lemma sort'_sorted : forall l1 l2, sorted l1 -> 
+  sorted (fst (sort' l1 l2)).
 Proof.
   fix sort'_sorted 2.
   intros l1. destruct l2. intros S.  simpl. apply S.
   intros S. 
   unfold sort', sort'_func. apply slide_sorted. simpl. snd. simpl. 
-  Print sort'_func. *)
+  Print sort'_func.
 
